Test/CommandTest.lean
@@ -46,7 +46,7 @@ import Runwai.Tactic
 }
 
 #runwai_prove Lookup := by {
-  rename_i Δ h_delta trace i hs hi ht he hty hσ σ Γ
+  rename_i Δ h_delta i hi Γ Η
   apply Ty.TypeJudgment.TE_LookUp; repeat rfl
   rw[← h_delta]
   simp
